---
layout: default
title: "Lecture 17: Recursion"
---

Recursive Functions
===================

> Often we can define a function that depends on a parameter *n* ∈ ℕ
*recursively* as

> *f*(0) = c

> ∀*n* ∈ ℕ, *f*(*n*+1) = *g*(*n*+1) *f*(*n*)

**Example 1**

> Consider the recursive function defined by

> *f*(0) = 1

> ∀*n* ∈ ℕ, *f*(*n*+1) = *f*(*n*) + 2<sup>n+1</sup>

This recursive function generates the sequence *f*(*n*) = 2<sup>0</sup> + 2<sup>1</sup> +
\... + 2<sup>n</sup> which we have previously seen computes to 2<sup>n+1</sup> - 1.

Rather than writing the sequence sum with an ellipsis, instead we
introduce the *summation* notation denoted by Σ. Thus the above sequence
can be written

> ![image](images/lecture17/sum.png)

and thus

> ![image](images/lecture17/sum2.png)

Often the limits of summation may not start at 0, thus we can generalize
the summation notation where the index ranges from *m* to *n* (clearly
*m* ≤ *n*) as

> ![image](images/lecture17/sumdiff.png)

Thus if we wished to compute the sum of the powers of 2 from 4 to 8

> ![image](images/lecture17/exsum.png)

**Example 2**

> Consider the recursive function defined by

> *f*(0) = 1

> ∀*n* ∈ ℕ, *f*(*n*+1) = (*n*+1) *f*(*n*)

As an example, to compute *f*(5) we would compute

> *f*(5) = 5 ⋅ *f*(4)
>
> > = 5 ⋅ 4 ⋅ *f*(3)
> >
> > = 5 ⋅ 4 ⋅ 3 ⋅ *f*(2)
> >
> > = 5 ⋅ 4 ⋅ 3 ⋅ 2 ⋅ *f*(1)
> >
> > = 5 ⋅ 4 ⋅ 3 ⋅ 2 ⋅ 1 ⋅ *f*(0)
> >
> > = 5 ⋅ 4 ⋅ 3 ⋅ 2 ⋅ 1 ⋅ 1
> >
> > = 120

This function is known as the *factorial* function and is denoted *n*!.
Thus 5! = 120. Similarly to the summation notation, we introduce
*product* notation denoted by Π. Thus the factorial function can be
written (noting that 0! = 1! = 1 and thus we can start the index at 1)

> ![image](images/lecture17/fact.png)

Unfortunately there is no closed form to compute *n*! although there are
approximations.

**Example 3**

> Prove that for *n* ≥ 4, *n*! \> 2<sup>n</sup>

Since both of these functions are defined recursively (note
exponentiation is simply repeated multiplication) we will attempt to
construct the proof using induction.

*Step 0:* Write the induction given closed form for *n*

> *n*! \> 2<sup>n</sup>

*Step 1:* Write the induction goal closed form for *n*+1

> (*n* + 1)! \> 2<sup>n+1</sup>

*Step 2:* Show the induction given is true for a base case

> Clearly for *n* = 4, *n*! = 24 \> 2<sup>4</sup> = 16.

*Step 3:* Factor the induction goal to include the induction given. **Note:** This is simply the *recursive* formula.

> (*n* + 1)! = (*n* + 1) ⋅ *n*!

*Step 4:* Assume the induction formula from step 0 is true and substitute the closed form solution into step 3.

> Therefore we *assume* *n*! \> 2<sup>n</sup>. Then

> (*n* + 1) ⋅ *n*! \> (*n* + 1) ⋅ 2<sup>n</sup>

*Step 5:* Perform any necessary algebra to show the closed form solution from step 1 for *n*+1

> (*n* + 1) ⋅ 2<sup>n</sup> \> 2 ⋅ 2<sup>n</sup>     (since (*n* + 1) \> 2 for *n* \> 4)
> > = 2<sup>n+1</sup>

Thus *n*! \> 2<sup>n</sup> for *n* ≥ 4.

**Example 4**

> Find a formula for the recursive sequence defined as

> *a*<sub>0</sub> = 0
>
> ∀*n* ∈ ℕ, *a*<sub>n+1</sub> = 2*a*<sub>n</sub> + n

Creating a table of values gives

> 
>  *n*    | *a*<sub>n</sub> |
> ------- | --------------- |
>   0     |         0       |
>   1     | 2⋅0+0=0         |
>   2     | 2⋅0+1=1         |
>   3     | 2⋅1+2=4         |
>   4     | 2⋅4+3=11        |
>   5     | 2⋅11+4=26       |
>   6     | 2⋅26+5=57       |

Hence we can guess a formula of the form *a*<sub>n</sub> = 2<sup>n</sup> - (n+1). To prove
this guess is correct we will use induction.

*Step 0:* Write the induction given closed form for *n*

> *a*<sub>n</sub> = 2<sup>n</sup> - (n+1)

*Step 1:* Write the induction goal closed form for *n*+1

> *a*<sub>n+1</sub> = 2<sup>n+1</sup> - ((n+1) + 1) = 2<sup>n+1</sup> - (n+2)

*Step 2:* Show the induction given is true for a base case

> For *n* = 0, 2<sup>0</sup> - (0+1) = 1 - 1 = 0.

*Step 3:* Factor the induction goal to include the induction given. **Note:** This is simply the *recursive* formula

> *a*<sub>n+1</sub> = 2*a*<sub>n</sub> + n

*Step 4:* Assume the induction formula from step 0 is true and substitute the closed form solution into step 3.

> Therefore we *assume* *a*<sub>n</sub> = 2<sup>n</sup> - (n+1). Then

> 2*a*<sub>n</sub> + n = 2(2<sup>n</sup> - (n+1)) + n

*Step 5:* Perform any necessary algebra to show the closed form solution from step 1 for *n*+1

> 2(2<sup>n</sup> - (n+1)) + n = 2<sup>n+1</sup> - 2*n* - 2 + n
> > = 2<sup>n+1</sup> - *n* - 1 - 1
> > 
> > = 2<sup>n+1</sup> - (*n*+2)
